LambdaS5/coq/LjsCorrectness.v
@@ -1200,16 +1200,21 @@ Proof.
     eauto using eval_correct.
 Qed.
 
-Lemma runs_lazy_correct : forall runs, runs_type_correct runs -> runs_type_correct (lazyruns (fun _ => runs)).
+Lemma runs_lazy_correct : forall runs, runs_type_correct runs -> runs_type_correct (suspend_runs (fun _ => runs)).
 Proof.
     introv IH.
     eapply make_runs_type_correct.
     eauto using runs_type_correct_eval. 
 Qed.
 
-Lemma runs_correct : forall k, runs_type_correct (runs k). 
+Lemma lazy_runs_correct : forall k, runs_type_correct (lazy_runs k). 
 Proof.
     induction k; eauto using runs_0_correct, runs_S_correct, runs_lazy_correct. 
+Qed.
+
+Lemma runs_correct : forall k, runs_type_correct (runs k). 
+Proof.
+    induction k; eauto using runs_0_correct, runs_S_correct. 
 Qed.
 
    
